

# Lecture 8: Polynomials in one variable II

## Remainder of the division by $x - a$

If  $f(x) = q(x)(x - a) + \text{remainder}$ , then we first observe that the remainder must be a number (degree 0). If the remainder degree has larger than 1, then we can continue dividing  $x - a$ .

**Example:** Consider  $x^2 + 1 / (x + 1)$ . The long division gives the remainder 2.

**Theorem:** The remainder equals  $f(a)$ . In particular, if  $f(a) = 0$ , then  $x - a$  divides  $f(x)$ .

**Proof:** When we plug  $a$  into the long division, we get  $f(a) = 0 + \text{remainder}$ . So the remainder is  $f(a)$ .

**Example revisited:**  $x + 1 = x - (-1)$ . So the remainder is  $f(-1) = (-1)^2 + 1 = 2$ .

**Example:**

- the remainder of  $x^2 - 3x + 2$  divides  $x - 2$  equals  $f(2) = 4 - 6 + 2 = 0$ .
- the remainder of  $x^2 - 3x + 2$  divides  $x - 1$  equals  $f(1) = 1 - 3 + 2 = 0$ .
- in other words,  $x - 1$  and  $x - 2$  both divides  $x^2 - 3x + 2$ . This is indeed the factorization

$$x^2 - 3x + 2 = (x - 1)(x - 2)$$

- Factorization of  $x^2 + 17x - 18$ . Consider  $f(1) = 1 + 17 - 18 = 0$ . So  $x - 1$  divides  $x^2 + 17x - 18$  and the factorization becomes  $x^2 + 17x - 18 = (x - 1)(x + 18)$ .

## Applications to factorizations

- $f(1)$  is the sum of all coefficients and  $f(-1)$  is the alternating sum of all coefficients of the polynomial. Those are always easy to check first when dealing with complicated factorization problems.
- Factorization of  $x^2 + 17x - 18$ . Consider  $f(1) = 1 + 17 - 18 = 0$ . So  $x - 1$  divides  $x^2 + 17x - 18$  and the factorization becomes  $x^2 + 17x - 18 = (x - 1)(x + 18)$ .
- Factorization of  $x^2 - 17x - 18$ . Consider  $f(-1) = 1 + 17 - 18 = 0$ . So  $x + 1$  divides  $x^2 - 17x - 18$  and the factorization becomes  $x^2 - 17x - 18 = (x + 1)(x + 18)$ .
- Factorization of  $x^3 - 3x - 2$ . Consider  $f(-1) = -1 + 3 - 2 = 0$ . So  $x + 1$  divides  $x^3 - 3x - 2 = (x + 1)(x^2 - x - 2) = (x + 1)^2(x - 2)$ . We can check  $f(2) = 0$  as well.

**Theorem:** a polynomial of degree  $d$  can have up to  $d$  roots.

**Proof:** If  $f(x)$  has a root  $a$ , then  $x - a$  divides  $f(x)$ . Now  $f(x) = (x - a)g(x)$ , where  $g(x)$  is a polynomial of degree  $d - 1$ . If  $f(x)$  has more than  $d$  roots, we do not enough degree to divide all of  $x - a_i$ .

**Examples:**

- $x^2 - 3x + 2$  has 2 roots
- $x^2 + 2x + 1$  has one (double) root
- $x^2 + 1$  has no root, but have two distinct complex roots  $x^2 + 1 = (x - \sqrt{-1})(x + \sqrt{-1}) = (x - i)(x + i)$ .
- $x^2 - 3x - 2$  has one double root and one simple root.
- $(x - 1)^n$  has one root with multiplicity  $n$ .
- $x^3 + 1 = (x + 1)(x^2 - x + 1)$  has one root and two complex roots.

**The Fundamental Theorem of Algebra (Gauss, the guy who did 1+2+...+100):** a polynomial of degree  $d$  have exactly  $d$  roots when counting multiplicities.

## Factorization of a polynomial

**Example:**

- $x^3 + x^2 + x + 1 = x^2(x + 1) + (x + 1) = (x^2 + 1)(x + 1)$ . You could also use  $f(-1) = 0$ .
- $x^5 + x^4 + \dots + x + 1 = (x^4 + x^2 + 1)(x + 1)$ . You could also use  $f(-1) = 0$ .
- $x^4 + 1 = x^4 + 2x^2 + 1 - 2x^2 = (x^2 + 1)^2 - 2x^2 = (x^2 + \sqrt{2}x + 1)(x^2 - \sqrt{2}x + 1)$ . No real roots at all.
- $x^5 + x + 1 = x^5 + x^4 + x^3 - x^4 - x^3 - x^2 + x^2 + x + 1 = (x^2 + x + 1)(x^3 - x^2 + 1)$ . This is tricky and we do not know if we could factorize  $x^3 - x^2 + 1$  any further.
- $x^n - 1 = (x - 1)(x^{n-1} + x^{n-2} + \dots + x + 1)$

**Examples to more variables:**

- $a^2 - b^2 = (a + b)(a - b)$
- $a^3 - b^3 = (a + b)(a^2 - ab + b^2)$
- $a^3 + b^3 = (a + b)(a^2 + ab + b^2)$
- $a^3 + b^3 + c^3 - 3abc = (a + b + c)(a^2 + b^2 + c^2 - ab - bc - ca)$ . This is really unexpected.

## Rational expressions

**Example:**

- $\frac{1}{(\frac{1}{a} + \frac{1}{b})/2} = \frac{2ab}{a+b}$ . Harmonic mean of two numbers: average speed with half on speed  $a$  and half on speed  $b$ .
- $\frac{1}{1 + \frac{1}{x}}$
- $\frac{\frac{1}{x}}{1 + \frac{1}{1 + \frac{1}{x}}}$

**Last fun example:**

$$\begin{aligned}
 & \frac{(x-a)(x-b)}{(c-a)(c-b)} + \frac{(x-a)(x-c)}{(b-a)(b-c)} + \frac{(x-b)(x-c)}{(a-b)(a-c)} \\
 &= \frac{(x-a)(x-b)(a-b) + (x-a)(x-c)(c-a) + (x-b)(x-c)(b-c)}{(a-b)(a-c)(b-c)} \\
 &= \frac{(a-b)x^2 - (a^2 - b^2)x + ab(a-b) + (c-a)x^2 - (c^2 - a^2)x + ac(c-a) + (b-c)x^2 - (b^2 - c^2)x + bc(b-c)}{(a-b)(a-c)(b-c)} \\
 &= \frac{a^2b - ab^2 + ac^2 - a^2c + b^2c - bc^2}{(a^2 - ab - ac + bc)(b-c)} \\
 &= \frac{a^2b - ab^2 + ac^2 - a^2c + b^2c - bc^2}{(a^2b - ab^2 - abc + bc^2 - a^2c + abc + ac^2 - bc^2)} = 1
 \end{aligned}$$